more functions private

examples/low-level/crypto/Crypto.Symmetric.AES.fst
@@ -29,13 +29,13 @@ type lbytes l = b:bytes {length b = l}
 let v (x:UInt32.t) : nat  = UInt32.v x
 
 (* Parameters for AES-256 *)
-inline_for_extraction let nb =  4ul 
-inline_for_extraction let nk =  8ul // 4, 6, or 8
-inline_for_extraction let nr = 14ul // 10, 12, or 14
+private inline_for_extraction let nb =  4ul 
+private inline_for_extraction let nk =  8ul // 4, 6, or 8
+private inline_for_extraction let nr = 14ul // 10, 12, or 14
 
-let blocklen = U32.(4ul *^ nb)
-let keylen   = U32.(4ul *^ nk)
-let xkeylen  = U32.(4ul *^ nb *^ (nr +^ 1ul)) // 176, 208, or 240
+private inline_for_extraction let blocklen = U32.(4ul *^ nb)
+private inline_for_extraction let keylen   = U32.(4ul *^ nk)
+private inline_for_extraction let xkeylen  = U32.(4ul *^ nb *^ (nr +^ 1ul)) // 176, 208, or 240
 
 type block = lbytes (v blocklen)
 type skey  = lbytes (v keylen)
@@ -44,11 +44,11 @@ type xkey  = lbytes (v xkeylen)
 type rnd = r:UInt32.t{v r <= v nr}
 type idx_16 = ctr:UInt32.t{v ctr <= 16}
 
-val xtime: b:byte -> Tot byte
+private inline_for_extraction val xtime: b:byte -> Tot byte
 let xtime b =
   (b <<^ 1ul) ^^ (((b >>^ 7ul) &^ 1uy) *%^ 0x1buy)
 
-val multiply: a:byte -> b:byte -> Tot byte
+private val multiply: a:byte -> b:byte -> Tot byte
 let multiply a b =
   ((a *%^ (b &^ 1uy))
   ^^ (xtime a *%^ ((b >>^ 1ul) &^ 1uy))
@@ -345,7 +345,7 @@ let mk_inv_sbox sbox =
   sbox.(252ul) <- 0x55uy; sbox.(253ul) <- 0x21uy; sbox.(254ul) <- 0x0cuy; sbox.(255ul) <- 0x7duy
 #reset-options
 
-let rec access_aux: sb:sbox -> byte -> ctr:UInt32.t{v ctr <= 256} -> byte -> STL byte
+private let rec access_aux: sb:sbox -> byte -> ctr:UInt32.t{v ctr <= 256} -> byte -> STL byte
   (requires (fun h -> live h sb))
   (ensures  (fun h0 _ h1 -> h1 == h0))
   = fun sbox i ctr tmp ->
@@ -354,7 +354,7 @@ let rec access_aux: sb:sbox -> byte -> ctr:UInt32.t{v ctr <= 256} -> byte -> STL
        let tmp = tmp |^ (mask &^ sbox.(ctr)) in
        access_aux sbox i (U32.(ctr +^ 1ul)) tmp
 
-val access: sb:sbox -> idx:byte -> STL byte
+private val access: sb:sbox -> idx:byte -> STL byte
   (requires (fun h -> live h sb))
   (ensures  (fun h0 _ h1 -> h1 == h0))
 let access sbox i =
@@ -364,7 +364,7 @@ let access sbox i =
 
 // ENCRYPTION 
 
-val subBytes_aux_sbox: state:block -> sb:sbox{disjoint state sb} -> ctr:idx_16 -> STL unit
+private val subBytes_aux_sbox: state:block -> sb:sbox{disjoint state sb} -> ctr:idx_16 -> STL unit
   (requires (fun h -> live h state /\ live h sb))
   (ensures  (fun h0 _ h1 -> live h1 state /\ modifies_1 state h0 h1))
 let rec subBytes_aux_sbox state sbox ctr =
@@ -376,13 +376,13 @@ let rec subBytes_aux_sbox state sbox ctr =
     subBytes_aux_sbox state sbox (U32.(ctr +^ 1ul))
   end
 
-val subBytes_sbox: state:block -> sbox:sbox{disjoint state sbox} -> STL unit
+private val subBytes_sbox: state:block -> sbox:sbox{disjoint state sbox} -> STL unit
   (requires (fun h -> live h state /\ live h sbox))
   (ensures  (fun h0 _ h1 -> modifies_1 state h0 h1 /\ live h1 state))
 let subBytes_sbox state sbox =
   subBytes_aux_sbox state sbox 0ul
 
-val shiftRows: state:block -> STL unit
+private val shiftRows: state:block -> STL unit
   (requires (fun h -> live h state))
   (ensures  (fun h0 _ h1 -> live h1 state /\ modifies_1 state h0 h1))
 let shiftRows state =
@@ -409,7 +409,7 @@ let shiftRows state =
   state.(i+^ 8ul) <- state.(i+^ 4ul);
   state.(i+^ 4ul) <- tmp
 
-val mixColumns_: state:block -> c:UInt32.t{v c < 4} -> STL unit
+private val mixColumns_: state:block -> c:UInt32.t{v c < 4} -> STL unit
   (requires (fun h -> live h state))
   (ensures  (fun h0 _ h1 -> live h1 state /\ modifies_1 state h0 h1))
 let mixColumns_ state c =
@@ -425,7 +425,7 @@ let mixColumns_ state c =
 
 #reset-options "--initial_fuel 0 --max_fuel 0"
 
-val mixColumns: state:block -> STL unit
+private val mixColumns: state:block -> STL unit
   (requires (fun h -> live h state))
   (ensures  (fun h0 _ h1 -> live h1 state /\ modifies_1 state h0 h1))
 let mixColumns state =
@@ -436,7 +436,7 @@ let mixColumns state =
 
 #reset-options "--z3rlimit 10 --initial_fuel 0 --max_fuel 0"
 
-val addRoundKey_: state:block -> w:xkey{disjoint state w} -> rnd -> c:UInt32.t{v c < 4} -> STL unit
+private val addRoundKey_: state:block -> w:xkey{disjoint state w} -> rnd -> c:UInt32.t{v c < 4} -> STL unit
   (requires (fun h -> live h state /\ live h w))
   (ensures  (fun h0 _ h1 -> live h1 state /\ modifies_1 state h0 h1))
 let addRoundKey_ state w round c =
@@ -449,7 +449,7 @@ let addRoundKey_ state w round c =
   target.(2ul) <- target.(2ul) ^^ subkey.(2ul);
   target.(3ul) <- target.(3ul) ^^ subkey.(3ul)
 
-val addRoundKey: state:block -> w:xkey{disjoint state w} -> round:rnd  -> STL unit
+private val addRoundKey: state:block -> w:xkey{disjoint state w} -> round:rnd  -> STL unit
   (requires (fun h -> live h state /\ live h w))
   (ensures  (fun h0 _ h1 -> live h1 state /\ modifies_1 state h0 h1))
 let addRoundKey state w round =
@@ -458,7 +458,7 @@ let addRoundKey state w round =
   addRoundKey_ state w round 2ul;
   addRoundKey_ state w round 3ul
 
-val cipher_loop: state:block -> w:xkey{disjoint state w} -> sb:sbox{disjoint sb state} -> round:rnd -> STL unit
+private val cipher_loop: state:block -> w:xkey{disjoint state w} -> sb:sbox{disjoint sb state} -> round:rnd -> STL unit
   (requires (fun h -> live h state /\ live h w /\ live h sb))
   (ensures  (fun h0 _ h1 -> live h1 state /\ modifies_1 state h0 h1))
 let rec cipher_loop state w sbox round =
@@ -493,7 +493,7 @@ let cipher out input w sbox =
 
 // KEY EXPANSION
 
-val rotWord: word:lbytes 4 -> STL unit
+private val rotWord: word:lbytes 4 -> STL unit
   (requires (fun h -> live h word))
   (ensures  (fun h0 _ h1 -> live h1 word /\ modifies_1 word h0 h1))
 let rotWord word =
@@ -506,7 +506,7 @@ let rotWord word =
   word.(2ul) <- w3;
   word.(3ul) <- w0
 
-val subWord: word:lbytes 4 -> sbox:sbox -> STL unit
+private val subWord: word:lbytes 4 -> sbox:sbox -> STL unit
   (requires (fun h -> live h word /\ live h sbox /\ disjoint word sbox))
   (ensures  (fun h0 _ h1 -> live h1 word /\ modifies_1 word h0 h1))
 let subWord word sbox =
@@ -517,7 +517,7 @@ let subWord word sbox =
 
 #reset-options "--z3rlimit 40 --initial_fuel 0 --max_fuel 0"
 
-val rcon: i:UInt32.t{v i >= 1} -> byte -> Tot byte (decreases (v i))
+private val rcon: i:UInt32.t{v i >= 1} -> byte -> Tot byte (decreases (v i))
 let rec rcon i tmp =
   if i = 1ul then tmp
   else begin
@@ -527,7 +527,7 @@ let rec rcon i tmp =
 
 #reset-options "--z3rlimit 20 --initial_fuel 0 --max_fuel 0"
 
-val keyExpansion_aux_0:w:xkey -> temp:lbytes 4 -> sbox:sbox -> i:UInt32.t{v i < (v xkeylen / 4) /\ v i >= v nk} -> STL unit
+private val keyExpansion_aux_0:w:xkey -> temp:lbytes 4 -> sbox:sbox -> i:UInt32.t{v i < (v xkeylen / 4) /\ v i >= v nk} -> STL unit
   (requires (fun h -> live h w /\ live h temp /\ live h sbox /\ 
                    disjoint w temp /\ disjoint w sbox /\ disjoint temp sbox))
   (ensures  (fun h0 _ h1 -> live h1 temp /\ modifies_1 temp h0 h1))
@@ -548,7 +548,7 @@ let keyExpansion_aux_0 w temp sbox j =
 
 #reset-options "--z3rlimit 50 --initial_fuel 0 --max_fuel 0"
 
-val keyExpansion_aux_1: w:xkey -> temp:lbytes 4 -> sbox:sbox -> i:UInt32.t{v i < (v xkeylen / 4) /\ v i >= v nk} -> STL unit
+private val keyExpansion_aux_1: w:xkey -> temp:lbytes 4 -> sbox:sbox -> i:UInt32.t{v i < (v xkeylen / 4) /\ v i >= v nk} -> STL unit
   (requires (fun h -> live h w /\ live h temp /\ live h sbox
     /\ disjoint w temp /\ disjoint w sbox /\ disjoint temp sbox))
   (ensures  (fun h0 _ h1 -> live h1 w /\ modifies_1 w h0 h1))
@@ -568,7 +568,7 @@ let keyExpansion_aux_1 w temp sbox j =
   w.(i+^2ul) <- H8.(t2 ^^ w2);
   w.(i+^3ul) <- H8.(t3 ^^ w3)
 
-val keyExpansion_aux: w:xkey -> temp:lbytes 4 -> sbox:sbox -> i:UInt32.t{v i <= (v xkeylen / 4) /\ v i >= v nk} -> STL unit
+private val keyExpansion_aux: w:xkey -> temp:lbytes 4 -> sbox:sbox -> i:UInt32.t{v i <= (v xkeylen / 4) /\ v i >= v nk} -> STL unit
   (requires (fun h -> live h w /\ live h temp /\ live h sbox
     /\ disjoint w temp /\ disjoint w sbox /\ disjoint temp sbox))
   (ensures  (fun h0 _ h1 -> live h1 temp /\ live h1 w /\ modifies_2 temp w h0 h1))
@@ -596,7 +596,7 @@ let keyExpansion key w sbox =
 
 // DECRYPTION
 
-val invSubBytes_aux_sbox: state:block -> sbox:sbox -> ctr:idx_16 -> STL unit
+private val invSubBytes_aux_sbox: state:block -> sbox:sbox -> ctr:idx_16 -> STL unit
   (requires (fun h -> live h state /\ live h sbox /\ disjoint state sbox))
   (ensures  (fun h0 _ h1 -> live h1 state /\ modifies_1 state h0 h1))
 let rec invSubBytes_aux_sbox state sbox ctr =
@@ -608,13 +608,13 @@ let rec invSubBytes_aux_sbox state sbox ctr =
     invSubBytes_aux_sbox state sbox (U32.(ctr+^1ul))
   end
 
-val invSubBytes_sbox: state:block -> sbox:sbox -> STL unit
+private val invSubBytes_sbox: state:block -> sbox:sbox -> STL unit
   (requires (fun h -> live h state /\ live h sbox /\ disjoint state sbox))
   (ensures  (fun h0 _ h1 -> live h1 state /\ modifies_1 state h0 h1))
 let invSubBytes_sbox state sbox =
   invSubBytes_aux_sbox state sbox 0ul
 
-val invShiftRows: state:block -> STL unit
+private val invShiftRows: state:block -> STL unit
   (requires (fun h -> live h state))
   (ensures  (fun h0 _ h1 -> live h1 state /\ modifies_1 state h0 h1))
 let invShiftRows state =
@@ -641,7 +641,7 @@ let invShiftRows state =
   state.(i+^8ul)  <- state.(i+^4ul);
   state.(i+^4ul)  <- tmp
 
-val invMixColumns_: state:block -> c:UInt32.t{v c < 4} -> STL unit
+private val invMixColumns_: state:block -> c:UInt32.t{v c < 4} -> STL unit
   (requires (fun h -> live h state))
   (ensures  (fun h0 _ h1 -> live h1 state /\ modifies_1 state h0 h1 ))
 let invMixColumns_ state c =
@@ -658,7 +658,7 @@ let invMixColumns_ state c =
 
 #reset-options "--initial_fuel 0 --max_fuel 0"
 
-val invMixColumns: state:block -> STL unit
+private val invMixColumns: state:block -> STL unit
   (requires (fun h -> live h state))
   (ensures  (fun h0 _ h1 -> live h1 state /\ modifies_1 state h0 h1 ))
 let invMixColumns state =
@@ -667,7 +667,7 @@ let invMixColumns state =
   invMixColumns_ state 2ul;
   invMixColumns_ state 3ul
 
-val inv_cipher_loop: state:block -> w:xkey -> sb:sbox -> round:UInt32.t{v round <= v nr - 1} -> STL unit
+private val inv_cipher_loop: state:block -> w:xkey -> sb:sbox -> round:UInt32.t{v round <= v nr - 1} -> STL unit
   (requires (fun h -> live h state /\ live h w /\ live h sb /\ disjoint state w /\ disjoint state sb /\ disjoint sb w))
   (ensures  (fun h0 _ h1 -> live h1 state /\ modifies_1 state h0 h1 ))
 let rec inv_cipher_loop state w sbox round =
